Progress toward hiding readers from R
Attempts to formalize notion that R doesn't read the disk's readers,
running into some trickiness coming up with a property that is general
enough and true of the cache locking discipline. The complexity should
mostly be hidden above the cache, where readers are irrelevant and
indeed can be hidden.

The current approach is to just have precise specs and simplify them at
a higher level, which could be sufficient depending on what we do.

src/ConcurrentCache.v
@@ -37,19 +37,6 @@ Module CacheTransitionSystem (Sem:Semantics) (CVars : CacheVars Sem).
   Definition GDisk := get HFirst stateVars.
   Definition GCache := get (HNext HFirst) stateVars.
 
-  (* TODO: replace with map for option *)
-  Definition mcache_get_lock (c:AssocCache BusyFlag) a :=
-    match (cache_state c a) with
-    | Some l => l
-    | None => Open
-    end.
-
-  Definition gcache_get_lock (c:AssocCache BusyFlagOwner) (a: addr) :=
-    match (cache_state c a) with
-    | Some l => l
-    | None => NoOwner
-    end.
-
   Definition get_m_lock (a: addr) (m: M Mcontents) :=
     mcache_get_lock (get Cache m) a.
 
@@ -93,7 +80,8 @@ Module CacheTransitionSystem (Sem:Semantics) (CVars : CacheVars Sem).
       let c := get Cache m in
       (d |= cache_pred c (get GDisk s))%judgement /\
       (* caches are equal, modulo relationship between real/ghost locks *)
-      cache_eq ghost_lock_invariant (get Cache m) (get GCache s).
+      cache_eq ghost_lock_invariant (get Cache m) (get GCache s) /\
+      reader_lock_inv (get GDisk s) (get GCache s).
 
 End CacheTransitionSystem.
 
@@ -102,9 +90,22 @@ on the definitions directly *)
 Hint Unfold lock_protects : prog.
 Hint Unfold StateR' : prog.
 
-Definition change_reader (vd: DISK) a rdr :=
+Definition rdr_dec : forall (rdr rdr': option ID), {rdr = rdr'} + {rdr <> rdr'}.
+Proof.
+  unfold ID.
+  decide equality.
+  decide equality.
+Defined.
+
+Lemma rdr_not_none : forall (rdr: option ID), rdr <> None ->
+                                         exists tid, rdr = Some tid.
+Proof.
+  destruct rdr; intros; (congruence || eauto).
+Qed.
+
+Definition change_reader (vd: DISK) a rdr' :=
   match vd a with
-  | Some (vs, _) => upd vd a (vs, rdr)
+  | Some (vs, _) => upd vd a (vs, rdr')
   | None => vd
   end.
 
@@ -137,11 +138,11 @@ Module Type CacheSemantics (Sem:Semantics) (CVars:CacheVars Sem).
     cacheR tid s' s'' ->
     R tid s s''.
 
-  Axiom relation_ignores_readers : forall tid (s s' s'': S Scontents) a rdr,
-      s' = set GDisk (change_reader (get GDisk s) a rdr) s ->
+  Axiom relation_ignores_readers : forall tid (s s' s'': S Scontents) a rdr',
+      s' = set GDisk (change_reader (get GDisk s) a rdr') s ->
       othersR R tid s' s'' ->
       exists s1, othersR R tid s s1 /\
-      s'' = set GDisk (change_reader (get GDisk s1) a rdr) s1.
+      s'' = set GDisk (change_reader (get GDisk s1) a rdr') s1.
 
 End CacheSemantics.
 
@@ -213,6 +214,30 @@ Ltac specific_addr :=
   | [ H: forall (_:addr), _, a: addr |- _ ] =>
     specialize (H a)
   end.
+
+Section Variables.
+
+Ltac vars_distinct :=
+  repeat rewrite member_index_eq_var_index;
+  repeat match goal with
+  | [ |- context[var_index ?v] ] => unfold v
+  end;
+  repeat erewrite get_hmap; cbn;
+  apply NoDup_get_neq with (def := 0); eauto;
+    autorewrite with hlist;
+    cbn; omega.
+
+Lemma GCache_neq_GDisk :
+  member_index GCache <> member_index GDisk.
+Proof.
+  vars_distinct.
+Qed.
+
+End Variables.
+
+Hint Immediate GCache_neq_GDisk.
+
+Hint Resolve not_eq_sym.
 
 Section CacheRTrans.
 
@@ -304,8 +329,6 @@ Proof.
   inversion H1; subst; eauto.
 Qed.
 
-Check lock_protects.
-
 Lemma lock_protects_indifference : forall lvar tv (v: _ -> tv) tid (s0 s0' s1 s1': S),
     lock_protects lvar v tid s0 s1 ->
     lvar s0 = lvar s0' ->
@@ -321,29 +344,48 @@ Proof.
   eauto.
 Qed.
 
-Section Variables.
-
-Ltac vars_distinct :=
-  repeat rewrite member_index_eq_var_index;
-  repeat match goal with
-  | [ |- context[var_index ?v] ] => unfold v
-  end;
-  repeat erewrite get_hmap; cbn;
-  apply NoDup_get_neq with (def := 0); eauto;
-    autorewrite with hlist;
-    cbn; omega.
-
-Lemma GCache_neq_GDisk :
-  member_index GCache <> member_index GDisk.
+Lemma same_domain_change_reader : forall d a rdr',
+    same_domain d (change_reader d a rdr').
 Proof.
-  vars_distinct.
+  unfold same_domain, subset, change_reader; intuition.
+  destruct matches;
+    distinguish_addresses; autorewrite with upd in *; eauto.
+  case_eq (d a); intros; simpl_match; eauto.
+  destruct w.
+  distinguish_addresses; autorewrite with upd in *; eauto.
 Qed.
 
-End Variables.
+Definition id_dec : forall (id1 id2:ID), {id1 = id2} + {id1 <> id2} :=
+  Nat.eq_dec.
 
-Hint Immediate GCache_neq_GDisk.
+Lemma cacheR_reader_collapse : forall tid (s s' s'' s''':S) vs0 a,
+    get GDisk s a = Some (vs0, None) ->
+    s' = set GDisk (change_reader (get GDisk s) a (Some tid)) s ->
+    reader_lock_inv (get GDisk s') (get GCache s') ->
+    othersR cacheR tid s' s'' ->
+    reader_lock_inv (get GDisk s'') (get GCache s'') ->
+    s''' = set GDisk (change_reader (get GDisk s'') a None) s'' ->
+    othersR cacheR tid s s'''.
+Proof.
+  unfold othersR, cacheR.
+  intros; subst.
+  deex; eexists; intuition eauto.
+  simpl_get_set in *.
+  eauto using same_domain_trans, same_domain_change_reader.
+  eapply lock_protocol_trans; [ eapply lock_protocol_trans | ];
+  [ | eapply H5 | ].
+  eapply lock_protocol_indifference; eauto.
+  unfold get_s_lock, gcache_get_lock; simpl_get_set.
+  eapply lock_protocol_indifference; eauto.
+  unfold get_s_lock, gcache_get_lock; simpl_get_set.
 
-Hint Resolve not_eq_sym.
+  match goal with
+  | [ H: forall (_:addr), _ |- _ ] => specialize (H a0); destruct_ands
+  end.
+
+  eapply lock_protects_indifference; eauto;
+  unfold get_s_lock, get_scache_val; now simpl_get_set.
+Abort.
 
 Lemma cacheR_ignores_readers : forall tid (s s' s'':S) a rdr,
     s' = set GDisk (change_reader (get GDisk s) a rdr) s ->
@@ -351,76 +393,7 @@ Lemma cacheR_ignores_readers : forall tid (s s' s'':S) a rdr,
     exists s1, othersR cacheR tid s s1 /\
           s'' = set GDisk (change_reader (get GDisk s1) a rdr) s1.
 Proof.
-  unfold change_reader, othersR, cacheR.
-  intros.
-  case_eq (get GDisk s a); intros.
-  - match goal with
-    | [ w: wr_set |- _ ] => destruct w
-    end.
-    deex.
-    repeat simpl_match.
-    simpl_get_set in *.
-    exists (set GDisk (change_reader (get GDisk s'') a o) s'').
-    unfold change_reader; simpl_get_set.
-    intuition.
-    eexists; intuition eauto.
-    * simpl_get_set.
-      eapply same_domain_remove_upd in H0; eauto.
-      case_eq (get GDisk s'' a); intros; eauto.
-      destruct w.
-      eauto using same_domain_trans, same_domain_upd.
-    * specialize (H4 a0); intuition.
-      eapply lock_protocol_indifference; eauto;
-      unfold get_s_lock, gcache_get_lock;
-      simpl_get_set.
-
-    * specialize (H4 a0); intuition.
-      unfold get_s_lock, get_scache_val in *.
-      eapply lock_protects_indifference; eauto; simpl_get_set.
-
-    * specialize (H4 a0); intuition.
-      unfold get_s_lock, get_disk_val in *.
-      unfold lock_protects; intros.
-      simpl_get_set.
-      specialize (H5 owner_tid); cbn in H5.
-      simpl_get_set in H5.
-      intuition.
-      distinguish_two_addresses a a0.
-      simpl_match; autorewrite with upd; auto.
-
-      autorewrite with upd in *.
-      case_eq (get GDisk s'' a); intros.
-      destruct w; autorewrite with upd; auto.
-      congruence.
-
-    * case_eq (get GDisk s'' a); intros;
-      try match goal with
-          | [ w: wr_set |- _ ] => destruct w
-          end;
-      simpl_get_set.
-      rewrite set_get; auto.
-      destruct matches; subst;
-      autorewrite with upd in *;
-      inv_opt.
-      eapply upd_same.
-
-      admit. (* seem to have lost a rdr; perhaps cache relation needs to say something about readers *)
-
-      assert (exists v, get GDisk s'' a = Some v).
-      eapply H0; autorewrite with upd; eauto.
-      deex; congruence.
-
-  - simpl_match.
-    simpl_get_set in H.
-    subst.
-    deex.
-    eexists; intuition eauto.
-    rewrite set_get; auto.
-    destruct matches.
-
-    eapply same_domain_none in H; eauto.
-    congruence.
-Qed.
+Abort.
 
 Theorem cacheR_trans_closed : forall tid (s s':S),
   star (cacheR tid) s s' ->
@@ -759,6 +732,7 @@ Hint Extern 4 (cache_pred _ _ _) => match goal with
 Hint Extern 4 (@eq (option _) _ _) => congruence.
 
 Definition locked_disk_read {T} a rx : prog Mcontents Scontents T :=
+  tid <- GetTID;
   c <- Get Cache;
   let val := match cache_get c a with
   | None => None
@@ -768,9 +742,9 @@ Definition locked_disk_read {T} a rx : prog Mcontents Scontents T :=
   end in
     match val with
     | None => v <- Read a;
-        let c' := cache_add c a v Open in
+        let c' := cache_add c a v Locked in
         GhostUpdate (fun s =>
-                    let vc' := cache_add (get GCache s) a v NoOwner in
+                    let vc' := cache_add (get GCache s) a v (Owned tid) in
                     set GCache vc' s);;
                     Assgn Cache c';;
                     rx v
@@ -800,7 +774,8 @@ Proof.
 Qed.
 
 Hint Resolve cache_vd_consistent_clean
-             cache_vd_consistent_dirty.
+     cache_vd_consistent_dirty
+     reader_lock_add_no_reader.
 
 Theorem locked_disk_read_ok : forall a,
     stateS TID: tid |-
@@ -829,7 +804,7 @@ Proof.
       simplify_step ||
       (time "inv_opt" inv_opt) ||
       (time "split_cache_val" split_cache_val) in
-      time "simplify" simplify' simp_step) with finish.
+     time "simplify" simplify' simp_step) with finish.
 Qed.
 
 Hint Extern 1 {{locked_disk_read _; _}} => apply locked_disk_read_ok : prog.
@@ -993,6 +968,18 @@ Qed.
 
 Hint Resolve addr_val_is.
 
+Hint Resolve reader_lock_add_reader
+     reader_lock_remove_reader.
+
+Lemma upd_ptsto_any : forall AT AEQ V (m: @mem AT AEQ V) a v,
+    (any * a |-> v)%pred (upd m a v).
+Proof.
+  intros.
+  eauto using any_sep_star_ptsto, upd_eq.
+Qed.
+
+Hint Resolve upd_ptsto_any.
+
 Theorem locked_AsyncRead_ok : forall a,
   stateS TID: tid |-
   {{ F v rest,
@@ -1004,12 +991,12 @@ Theorem locked_AsyncRead_ok : forall a,
                    R tid s0 s
    | POST d' m' s0' s' r: let vd' := virt_disk s' in
                           Inv m' s' d' /\
-                          (exists F', vd' |= F' * a |-> (Valuset v rest, None)) /\
-                          (* not quite true, since first need a step
-                            to add the reader and need a step at the
-                            end to remove it, which cannot be
-                            performed under othersR R *)
-                          star (othersR R tid) s s' /\
+                          (vd' |= any * a |-> (Valuset v rest, None)) /\
+                          star (othersR R tid)
+                               (set GDisk (change_reader (get GDisk s)
+                                                         a (Some tid)) s)
+                               (set GDisk (change_reader (get GDisk s')
+                                                         a (Some tid)) s') /\
                           cache_get (get Cache m') a = Some (Invalid Locked) /\
                           get_s_lock a s' = Owned tid /\
                           r = v /\
@@ -1035,43 +1022,40 @@ Proof.
   time "step" step pre (time "simplify" simplify) with finish.
 
   assert (get GDisk s2 a = Some (Valuset v rest, Some tid)).
-  (* H16 is star from a modified s to the current state s2 *)
-  eapply virt_disk_addr_readonly in H16; eauto.
-  rewrite H16.
+  (* H17 is star from a modified s to the current state s2 *)
+  eapply virt_disk_addr_readonly in H17; eauto.
+  rewrite H17.
   simpl_get_set.
-  autorewrite with upd; auto.
+  autorewrite with upd; now auto.
 
-  eapply cache_addr_readonly in H16; eauto.
-  unfold get_scache_val, opt_cache_entry_val in H16.
-  simpl_get_set in H16.
-  assert (cache_get (get GCache s) a = Some (Invalid (Owned tid))).
-  eauto using cache_eq_invalid.
+  eapply cache_addr_readonly in H17; eauto.
+  simpl_get_set in H17.
+  assert (cache_get (get GCache s) a = Some (Invalid (Owned tid))) by
+      eauto using cache_eq_invalid.
 
   assert (cache_get (get Cache m0) a = Some (Invalid Locked)).
-  eapply cache_eq_mem in H21; eauto; simplify.
+  eapply cache_eq_mem in H17; eauto; simplify.
   eauto.
   assert (get GDisk s2 a = d1 a) by eauto using cache_miss_mem_eq.
   assert (d1 a = Some (Valuset v rest, Some tid)) by eauto.
-
-  eapply addr_val_is; eauto.
+  eauto.
 
   (* TODO: forward chain this rather than copy it *)
 
   assert (get GDisk s2 a = Some (Valuset v rest, Some tid)).
-  (* H16 is star from a modified s to the current state s2 *)
-  eapply virt_disk_addr_readonly in H16; eauto.
-  rewrite H16.
+  (* H17 is star from a modified s to the current state s2 *)
+  eapply virt_disk_addr_readonly in H17; eauto.
+  rewrite H17.
   simpl_get_set.
-  autorewrite with upd; auto.
+  autorewrite with upd; now auto.
 
-  eapply cache_addr_readonly in H16; eauto.
-  unfold get_scache_val, opt_cache_entry_val in H16.
-  simpl_get_set in H16.
-  assert (cache_get (get GCache s) a = Some (Invalid (Owned tid))).
-  eauto using cache_eq_invalid.
+  eapply cache_addr_readonly in H17; eauto.
+  simpl_get_set in H17.
+  assert (cache_get (get GCache s) a = Some (Invalid (Owned tid))) by
+      eauto using cache_eq_invalid.
 
   assert (cache_get (get Cache m0) a = Some (Invalid Locked)).
-  eapply cache_eq_mem in H21; eauto; simplify.
+  eapply cache_eq_mem in H17; eauto; simplify.
   eauto.
   assert (get GDisk s2 a = d1 a) by eauto using cache_miss_mem_eq.
   assert (d1 a = Some (Valuset v rest, Some tid)) by eauto.
@@ -1081,20 +1065,20 @@ Proof.
   time "step" step pre (time "simplify" simplify) with finish.
   time "step" step pre (time "simplify" simplify) with finish.
 
-  apply diskIs_combine_upd in H27; unfold diskIs in H27; subst.
+  match goal with
+    | [ H: (diskIs _ * ?a |-> _)%pred ?d |- _ ] =>
+      apply diskIs_combine_upd in H; unfold diskIs in H; subst
+  end.
   eauto.
 
-  apply diskIs_split_upd; eauto.
-
-  (* spec needs to be updated to deal with fact that before yielding,
-  we set a reader *)
-  admit.
+  simpl_get_set in *.
+  unfold change_reader.
+  autorewrite with upd; simplify.
+  rewrite set_get with (l := s2) by auto.
+  auto.
 
   unfold get_s_lock in *.
-  simplify.
-  unfold gcache_get_lock.
-  rewrite cache_state_as_get.
-  simplify.
+  simplify; eauto.
 
   eapply star_one_step.
   eapply cache_relation_preserved; eauto.
@@ -1102,14 +1086,13 @@ Proof.
   unfold cacheR; simplify; eauto.
   unfold get_scache_val; simplify.
   unfold get_disk_val; simplify.
-  distinguish_addresses; eauto.
+  distinguish_addresses; autorewrite with upd; eauto.
   assert (get_s_lock a0 s2 = Owned tid).
   unfold get_s_lock, gcache_get_lock.
   rewrite cache_state_as_get.
   simplify.
   congruence. (* contradiction with tid <> owner_tid *)
-  autorewrite with upd; auto.
-Admitted.
+Qed.
 
 Hint Extern 4 {{ locked_AsyncRead _; _ }} => apply locked_AsyncRead_ok : prog.
 
